src/ReadOnlyFS.v
@@ -3,18 +3,50 @@ Require Import CoopConcurAuto.
 Require ConcurrentCache.
 Require Import Protocols.
 Require Import ConcurrentFS.
+Require Import Rec.
+Require Import DirTree.
 
 Import Hlist.
 Import Hlist.HlistNotations.
 Open Scope hlist_scope.
 
+Require Import GenSepN BFile Log SuperBlock.
+Require Import ConcurrentBridge.
+
+(** TODO:
+
+add mscs and fsxp to memory state and pass them to file system code from memory
+
+write the read-only invariant (factor out common part of specs) and protocol
+(trivial - fsxp and directory don't change) *)
+
 Module St <: GlobalState.
-  (* TODO: add file-system state *)
-  Definition Sigma := ConcurrentCache.Sigma.
+  Definition Sigma :=
+    defState (mem_types ConcurrentCache.Sigma ++
+                        (BFILE.memstate
+                           :: (FSLayout.fs_xparams:Type)
+                           :: nil))
+             (abstraction_types ConcurrentCache.Sigma ++
+                                ((FSLayout.fs_xparams:Type)
+                                   :: DIRTREE.dirtree
+                                   :: nil)).
 End St.
 
 Arguments HNext {A elm a types} _.
 Notation "f @ x" := (f x) (at level 10, x at level 20, only parsing).
+
+Definition mMscs : var (mem_types St.Sigma) BFILE.memstate :=
+  HNext @ HNext @ HFirst.
+
+Definition mFsxp : var (mem_types St.Sigma) FSLayout.fs_xparams :=
+  HNext @ HNext @ HNext @ HFirst.
+
+Definition vFsxp : var (abstraction_types St.Sigma) FSLayout.fs_xparams :=
+  HNext @ HNext @ HNext @ HNext @ HNext @ HFirst.
+
+Definition vDirTree : var (abstraction_types St.Sigma) DIRTREE.dirtree :=
+  HNext @ HNext @ HNext @ HNext @ HNext @ HNext @ HFirst.
+
 Hint Constructors List.NoDup.
 
 Ltac prove_nodup :=
@@ -43,19 +75,36 @@ Module CacheProj <: ConcurrentCache.CacheProj St.
   Defined.
 End CacheProj.
 
-
 Module CacheSubProtocol <: ConcurrentCache.CacheSubProtocol.
   Module CacheProtocol := ConcurrentCache.MakeCacheProtocol St CacheProj.
 
   Module App <: GlobalProtocol.
     Module St := St.
     Definition Sigma := St.Sigma.
+
     (* this won't be so simple with additional state in Sigma *)
     Definition delta : Protocol Sigma.
       apply (defProtocol
-             (fun d m s => invariant CacheProtocol.delta d m s)
-             (fun tid s s' => guar CacheProtocol.delta tid s s')).
-      apply guar_preorder.
+               (fun d m s =>
+                  invariant CacheProtocol.delta d m s /\
+                  let fsxp := get mFsxp m in
+                  let mscs := get mMscs m in
+                  let tree := get vDirTree s in
+                  (* TODO: eventually hm should be part of invariant *)
+                  exists ds hm ilist frees,
+                    LOG.rep (FSLayout.FSXPLog fsxp) (SB.rep fsxp)
+                            (LOG.NoTxn ds) (BFILE.MSLL mscs) hm
+                            (lower_disk (get CacheProtocol.vdisk s)) /\
+                    ((DIRTREE.rep fsxp emp tree ilist frees)
+                       @ list2nmem (ds!!))%pred /\
+                    get vFsxp s = fsxp)
+               (fun tid s s' => guar CacheProtocol.delta tid s s' /\
+                             get vDirTree s' = get vDirTree s /\
+                             get vFsxp s' = get vFsxp s)).
+      intros; constructor; hnf; intros.
+      intuition idtac; apply guar_preorder.
+      intuition idtac; try congruence.
+      eapply guar_preorder; eauto.
     Defined.
   End App.
 
@@ -63,8 +112,26 @@ Module CacheSubProtocol <: ConcurrentCache.CacheSubProtocol.
 
   Definition protocolProj:SubProtocol App.delta CacheProtocol.delta.
   Proof.
-    constructor; intros; eauto.
+    constructor; simpl; intros; intuition idtac.
   Qed.
+
+  Ltac unmodified_var :=
+    try match goal with
+        | [ H: modified _ ?l ?l' |- get _ ?l' = get _ ?l ] =>
+          symmetry; apply H
+        end;
+    try match goal with
+        | [ H: modified _ ?l ?l' |- get _ ?l = get _ ?l' ] =>
+          apply H
+        end;
+    match goal with
+    | [ |- HIn _ _ -> False ] =>
+      solve [ intros;
+              repeat match goal with
+                     | [ H: HIn _ _ |- _ ] =>
+                       inversion H; subst; repeat sigT_eq; clear H
+                     end ]
+    end.
 
   Definition protocolRespectsPrivateVars :
     forall tid s s',
@@ -72,8 +139,9 @@ Module CacheSubProtocol <: ConcurrentCache.CacheSubProtocol.
       modified [( CacheProtocol.vCache; CacheProtocol.vDisk0 )] s s' ->
       guar App.delta tid s s'.
   Proof.
-    intros.
-    eauto.
+    simpl; intros; intuition idtac.
+    unmodified_var.
+    unmodified_var.
   Qed.
 
   Definition invariantRespectsPrivateVars :
@@ -84,12 +152,21 @@ Module CacheSubProtocol <: ConcurrentCache.CacheSubProtocol.
       invariant CacheProtocol.delta d' m' s' ->
       invariant App.delta d' m' s'.
   Proof.
-    intros.
-    eauto.
+    simpl; intuition idtac.
+    repeat deex.
+    assert (get mFsxp m' = get mFsxp m) as Hfsxp by unmodified_var.
+    assert (get mMscs m' = get mMscs m) as Hmscs by unmodified_var.
+    assert (get CacheProtocol.vdisk s' = get CacheProtocol.vdisk s) as Hvdisk by unmodified_var.
+    assert (get vDirTree s' = get vDirTree s) as Htree by unmodified_var.
+    assert (get vFsxp s' = get vFsxp s) as Hvfsxp by unmodified_var.
+    unfold id in *; simpl in *.
+    rewrite !Hfsxp, !Hmscs, !Hvdisk, !Htree, !Hvfsxp in *.
+    repeat match goal with
+           | |- exists _, _ => eexists
+           end.
+    intuition eauto.
   Qed.
 
 End CacheSubProtocol.
 
 Module CFS := ConcurFS CacheSubProtocol.
-
-Print CFS.
